coq/Machine2.v
@@ -1,0 +1,93 @@
+Require Import Coq.Program.Program.
+Require Import Coq.Strings.String.
+Require Import Coq.Vectors.Vector.
+Require Import Coq.Lists.List.
+Require Import Coq.Sets.Ensembles.
+
+Section Scenarios.
+  (* Data state. Information that is global to a machine--and so visible outside
+  of a scenario. *)
+  Variable DState : Type.
+  (* Input events *)
+  Variable IEvent : Type.
+  (* Output events *)
+  Variable OEvent : Type.
+  (* Internal events *)
+  Variable MEvent : Type.
+
+  Record Scenario :=
+    mkScenario
+      { (* Machine state. I.e. Q in a normal state machine. *)
+        MState : Type;
+        start_state : MState;
+        error_state : MState;
+        transition :
+          MState -> DState -> (IEvent + OEvent + MEvent) -> MState;
+        dstate_update :
+          MState -> DState -> (IEvent + OEvent + MEvent) -> DState;
+        output :
+          MState -> DState -> (IEvent + OEvent + MEvent) ->
+          list (IEvent + OEvent + MEvent);
+
+        (* Error state properties *)
+        error_state_distinct : error_state <> start_state;
+        error_event : OEvent;   (* TODO name location of error *)
+        error_state_stuck : forall ds ie,
+          transition error_state ds ie = error_state;
+        error_state_silent : forall ds ie,
+          output error_state ds ie = nil;
+        error_state_idempotent : forall ds ie,
+          dstate_update error_state ds ie = ds;
+        error_state_entry : forall ms ds ie,
+            transition ms ds ie = error_state ->
+            output ms ds ie = error_event::nil;
+      }.
+
+  Record ScenarioConfig (S : Scenario) :=
+    mkScenarioConfig
+      { sc_mstate : MState S;
+        sc_dstate : DState;
+        sc_ievents : list IEvent;
+      }.
+
+  Arguments sc_mstate {_} _.
+  Arguments sc_dstate {_} _.
+  Arguments sc_ievents {_} _.
+
+  Inductive MicroStep (S : Scenario) (sc1 sc2 : ScenarioConfig S) : Prop :=
+  | MicroStep_basic : forall ie ms2,
+      transition S (sc_mstate sc1) (sc_dstate sc1) ie = sc_mstate sc2 ->
+      dstate_update S (sc_mstate sc1) (sc_dstate sc1) ie = sc_dstate sc2 ->
+      List.In ie (sc_ievents sc1) ->
+      (sc_ievents sc2) = (sc_ievents sc1) \\ ie ∪ (output S ...) ->
+      output S (sc_mstate sc1) (sc_dstate sc1) ie = ms2 ->
+      (sc_mstate sc2) <> error_state S ->
+      MicroStep S sc1 sc2.
+
+  .
+End Scenarios.
+
+Section Machines.
+  Variable State : Type.
+  Variable DataState : Type.
+  Variable InputEvent : Type.
+  Variable OutputEvent : Type.
+  Variable InternalEvent : Type.
+
+  Record Machine :=
+    mkMachine
+      { initial : State;
+        transition :
+          State -> DataState -> InputEvent -> State * DataState;
+        output :
+          State -> DataState -> InputEvent -> list (OutputEvent + InternalEvent);
+        error_state : State;
+        no_update_on_err : forall s d σ d',
+            transition s d σ = (error_state, d') -> d = d';
+        no_output_on_err : forall s d σ,
+            transition s d σ = (error_state, d) -> output s d σ = nil;
+      }.
+
+  Record Configuration :=
+    mkConfiguration
+      { S
