coq/Semantics.v
@@ -1,8 +1,10 @@
+Require Import Coq.Program.Program.
 Require Import Coq.Strings.String.
 Require Import Coq.QArith.QArith.
 Require Import Coq.Vectors.Vector.
 Require Import Coq.Lists.List.
 Require Import Coq.Sets.Ensembles.
+Require Import SMEDL.Util.
 Require Import SMEDL.Types.
 Require Import SMEDL.AST.
 Require SMEDL.VarEnv.
@@ -16,6 +18,7 @@ Require Import SMEDL.Machine.
 
 Arguments exist {_ _} _ _.
 Arguments existT {_ _} _ _.
+Arguments Empty_set {_ _}.
 
 Fixpoint compile_type (ty : Ty) : Set :=
   match ty with
@@ -25,29 +28,133 @@ Fixpoint compile_type (ty : Ty) : Set :=
   | SProduct lhs rhs => compile_type lhs * compile_type rhs
   end.
 
-Program Fixpoint LM_state'
-         (gs : list GlobalDecl)
-         (Γ : VarEnv.t)
-         (Hty : HasTy_VarEnv gs Γ) : Type :=
-  match gs with
-  | List.nil => unit
-  | (n,ty)::gs' => compile_type ty
-                   * LM_state' gs'
-                               (VarEnv.remove Γ n)
-                               (VarEnv_shrink n Hty)
+Fixpoint initial_value (ty : Ty) : (compile_type ty) :=
+  match ty with
+  | SInt => 0%nat
+  | SBool => false
+  | SFloat => 0%Q
+  | SProduct lhs rhs => (initial_value lhs, initial_value rhs)
   end.
+
+Program Definition GlobalDecls_global_state (gs : list GlobalDecl) : Type :=
+  forall (v : { n : string | List.In n (List.map fst gs) }),
+    compile_type (lookup string_dec v gs _).
+
+Program Fixpoint SM_states (sm : Scenario) : Ensemble string :=
+  fun x => List.In x (app (List.map Transition_source sm)
+                          (List.map Transition_dest sm)).
+
+Definition SM_state (gs : list GlobalDecl) (sm : Scenario) : Type :=
+  { n : string | In (SM_states sm) n } * GlobalDecls_global_state gs.
+
+(* e is the tag that tells you which event. It is paired with a function from
+   parameter names to values of the correct types for the parameters. *)
+Program Definition EventDecls_events (es : list EventDecl) : Type :=
+  { e : { n : string | List.In n (List.map fst es) } &
+        let ps := lookup string_dec e es _ in
+        forall p : { n : string | List.In n (List.map fst ps) },
+          compile_type (lookup string_dec p ps _) }.
+
+Program Definition GlobalDecls_initial_state
+        (gs : list GlobalDecl) : GlobalDecls_global_state gs :=
+  fun p => initial_value (lookup string_dec p gs _).
+
+Program Definition transition_starts_with (src : string) (t : Transition) : bool :=
+  Sumbool.bool_of_sumbool (string_dec src (Transition_source t)).
+
+(*
+Program Fixpoint eval_expr
+        {ty : Ty}
+        {gs : list GlobalDecl}
+        {es : list EventDecl}
+        (s : GlobalDecls_global_state gs)
+        (σ : EventDecls_events es)
+         (Γ : VarEnv.t)
+        (HΓ : HasTy_VarEnv gs Γ)
+        (expr : Expr)
+        (Hsm : HasTy_Expr Γ expr ty) : compile_type ty :=
+  match ty with
+  | SInt => match expr with
+            | LitInt n => n
+            | Var v => _
+            | UnOpExpr op body => eval_expr s σ _ HΓ body _
+            | BinOpExpr op lhs rhs => _
+            | _ => _
+            end
+  | SFloat => match expr with
+              | LitFloat q => q
+              | _ => _
+              end
+  | SBool => match expr with
+             | LitBool b => b
+             | _ => _
+             end
+  | _ => _
+  end.
+(* there has to be a better way to do this... in particular, I want to be able
+to specify (s v) up front, and only use Ltac to prove the type conversion. *)
 Obligation 1.
-inversion Hty as [_ Hdom _].
-specialize (Hdom n).
-inversion Hdom.
-eauto using in_eq.
-Qed.
+unfold GlobalDecls_global_state in s.
+assert (List.In v (map fst gs)) as Hin.
+{ inversion Hsm; subst.
+  destruct v0.
+  simpl.
+  inversion HΓ as [_ Hdom _].
+  specialize (Hdom x).
+  inversion Hdom as [Hdom' _].
+  specialize (Hdom' i).
+  inversion Hdom'.
+  apply (List.in_map fst) in H.
+  simpl in H.
+  exact H.
+}
+specialize (s (exist v Hin)).
+simpl in s.
+assert (compile_type (lookup string_dec v gs Hin) = nat).
+{
+  inversion Hsm; subst.
+  destruct v0.
+  inversion HΓ as [? Hdom Hlookup].
+  specialize (Hdom x).
+  inversion Hdom as [Hin_maps Hmaps_in].
+  specialize (Hin_maps i).
+  inversion_clear Hin_maps as [ty Hdom_in].
+  admit.
+}
+rewrite H in s.
+exact s.
+Admitted.
 
-(* Program Definition LM_state (lm : LocalMonitor) (Hty : HasTy_LM lm) : Type := *)
-(*   LM_state' (globals lm) _ _. *)
+Program Definition SM_transition
+        {gs : list GlobalDecl}
+        {es : list EventDecl}
+        (sm : Scenario)
+        (s : SM_state gs sm)
+        (σ : EventDecls_events es)
+        (Δ : EventEnv.t)
+        (HΔ : HasTy_EventEnv es Δ)
+        (Γ : VarEnv.t)
+        (HΓ : HasTy_VarEnv gs Γ)
+        (Hsm : HasTy_Scenario Δ Γ sm) : option (SM_state gs sm) :=
+  let (src,_) := s in
+  let ts := filter (transition_starts_with src) sm in
+  let t := find (guard_passes s) ts in
+  (Transition_dest t, (eval_command t) s).
 
-(* Definition LM_input (lm : LocalMonitor) : Type := *)
-(*   lm . *)
+Program Definition LM_output
+        (lm : LocalMonitor)
+        (Hlm : HasTy_LM lm)
+        (s : LM_state lm)
+        (σ : LM_input_events lm) : LM_input_events lm :=
+  _.
 
-(* Definition LM_output (lm : LocalMonitor) : Type := *)
-(*   lm . *)
+Definition LM_machine
+        (lm : LocalMonitor)
+        (Hlm : HasTy_LM lm)
+  : Machine (LM_input_events lm) (LM_output_events lm) :=
+  mkMachine
+    (LM_state lm)
+    (LM_initial_state lm)
+    (LM_transition lm Hlm)
+    (LM_output lm Hlm).
+*)
