coq/Util.v
@@ -1,0 +1,59 @@
+Require Import Coq.Lists.List.
+Require Import Coq.Program.Program.
+Require Import Coq.Sets.Ensembles.
+
+Arguments In {_} _ _.
+Arguments Add {_} _ _ _.
+
+Program Definition extend
+        {A : Type}
+        {B : Type}
+        {A_dec : forall (x y : A), {x = y} + {x <> y}}
+        {ps : Ensemble A}
+        (f : {x : A | In ps x} -> B)
+        (a : A)
+        (b : B)
+        (x : { x : A | In (Add ps a) x }) : B :=
+  if A_dec a x
+  then b
+  else f x.
+Obligation 1.
+inversion H0; subst; auto.
+inversion H1.
+contradiction.
+Qed.
+
+Fixpoint lookup_option
+        {A B : Type}
+        (A_dec : forall (x y : A), { x = y } + { x <> y })
+        (x : A)
+        (xys : list (A * B)) : option B :=
+  match xys with
+  | nil => None
+  | (x',y)::xys' =>
+    if A_dec x x'
+    then Some y
+    else lookup_option A_dec x xys'
+  end.
+
+Program Definition lookup
+        {A B : Type}
+        (A_dec : forall (x y : A), { x = y } + { x <> y })
+        (x : A)
+        (xys : list (A * B))
+        (Hin : List.In x (List.map fst xys)) : B :=
+  match lookup_option A_dec x xys with
+  | Some x' => x'
+  | None => _
+  end.
+Obligation 1.
+exfalso.
+induction xys.
+inversion Hin.
+destruct a; simpl in *.
+destruct (A_dec x a); subst; simpl in *.
+inversion Heq_anonymous.
+apply IHxys.
+inversion Hin; subst; try congruence.
+auto.
+Qed.
